Fixed pearlite

examples/pearlite-example/src/pearlite_example.rs
@@ -6,11 +6,11 @@ use hacspec_lib::*;
 #[cfg(not(feature = "hacspec"))]
 use creusot_contracts::{ensures, requires};
 
-#[ensures(result == result)]
+#[ensures(result == true)]
 #[cfg(test)]
 #[proof]
 #[quickcheck]
 pub fn ensure_something (x : u8, y : u8) -> bool {
-    true
+    x == y
 }
 
