coq/_vc/Pearlite_Example.v
@@ -11,11 +11,11 @@ Require Import QuickChickLib.
 Require Import Hacspec_Lib.
 
 Definition ensure_something (x_0 : int8) (y_1 : int8)  : bool :=
-  true.
+  (x_0) =.? (y_1).
 
 Theorem ensures_ensure_something : forall result_2 (x_0 : int8) (y_1 : int8),
  @ensure_something x_0 y_1 = result_2 ->
- result.
+ result_2 = true.
  Proof. Admitted.
 (*QuickChick (
   forAll g_int8 (fun x_0 : int8 =>forAll g_int8 (fun y_1 : int8 =>ensure_something x_0 y_1))).*)
