coq/src/Pearlite_Example.v
@@ -8,3 +8,16 @@ Open Scope bool_scope.
 Open Scope hacspec_scope.
 From QuickChick Require Import QuickChick.
 Require Import QuickChickLib.
+Require Import Hacspec_Lib.
+
+Definition ensure_something (x_0 : int8) (y_1 : int8)  : bool :=
+  (x_0) =.? (y_1).
+
+Theorem ensures_ensure_something : forall result_2 (x_0 : int8) (y_1 : int8),
+ @ensure_something x_0 y_1 = result_2 ->
+ result_2 = true.
+ Proof. Admitted.
+(*QuickChick (
+  forAll g_int8 (fun x_0 : int8 =>forAll g_int8 (fun y_1 : int8 =>ensure_something x_0 y_1))).*)
+
+
